theories/string_lang/StringLang.v
@@ -15,7 +15,7 @@ Definition string := list nat.
 Inductive statement : Type :=
   | APPEND: nat -> variable -> statement
   | DEL : variable -> statement
-  | IF_ENDS_GOTO   : variable -> nat -> option label -> statement.
+  | IF_ENDS_GOTO   : variable -> nat -> label -> statement.
 
 Inductive instruction : Type :=
   | Instr : option label -> statement  -> instruction.
@@ -55,11 +55,11 @@ Definition eq_inst_label  (instr : instruction ) (opt_lbl : option label) :=
   | Instr opt_lbl' _ => eqb_opt_lbl opt_lbl' opt_lbl
   end.
 
-Fixpoint get_labeled_instr (p : program) (lbl : option label) : nat :=
+Fixpoint get_labeled_instr (p : program) (lbl : label) : nat :=
   match p with
   | [] => 0
   | h :: t =>
-      if eq_inst_label h lbl
+      if eq_inst_label h (Some lbl)
       then 0
       else 1 + get_labeled_instr t lbl
   end.
